\subsubsection{Exercise} 

The RGA of the system at frequency 0 is:
$$
\text{RGA}(G(0)) = G(0).\ast[G^{-1}(0)]^T 
$$

With:

\begin{equation*}
    G(0) =
\left[
    \begin{array}{cc}
        \gamma_1k_1c_1 & (1-\gamma_2)k_2c_1 \\
        (1-\gamma_1)k_1c_2 & \gamma_2k_2c_2 \\
    \end{array}
\right]
\end{equation*}
\begin{multline*}
[G^{-1}(0)]^T = \\
\frac{1}{k_1k_2c_1c_2(\gamma_1+\gamma_2-1)}
\left[
    \begin{array}{cc}
        \gamma_2k_2c_2 & -(1-\gamma_1)k_1c_2 \\
        -(1-\gamma_2)k_2c_1 & \gamma_1k_1c_1 \\
    \end{array}
\right]\\
\end{multline*}
\begin{multline*}
    \text{RGA}(G(0)) =\\ 
\frac{1}{\gamma_1+\gamma_2-1}
\left[
    \begin{array}{cc}
        \gamma_1\gamma_2 & -(1-\gamma_1)(1-\gamma_2) \\
        -(1-\gamma_1)(1-\gamma_2) & \gamma_1\gamma_2 \\
    \end{array}
\right]
\end{multline*}

\begin{equation}
    \boxed{
    \text{RGA}(G(0)) =
    \left[
        \begin{array}{cc}
            \lambda & 1 - \lambda \\
            1 - \lambda & \lambda
        \end{array}
    \right]
}
\end{equation}

Where $\lambda = \frac{\gamma_1\gamma_2}{\gamma_1+\gamma_2-1}$.
